Batteries.lean
@@ -22,6 +22,7 @@ import Batteries.Data.ByteArray
 import Batteries.Data.Char
 import Batteries.Data.DList
 import Batteries.Data.Fin
+import Batteries.Data.FloatArray
 import Batteries.Data.HashMap
 import Batteries.Data.Int
 import Batteries.Data.LazyList
